examples/pseudo_bool/cp_encoding/cp_to_ilp_primScript.sml
@@ -46,6 +46,16 @@ Definition encode_equal_def:
     abstr (cencode_equal_2 bnd Zc X Y name)
 End
 
+Theorem lit_reify_avar_reif_gen:
+  lit (reify_avar cs wi) (reif_gen (Z,cmp,v)) ⇔
+    cmpop_val cmp (varc wi Z) v
+Proof
+  simp[reif_gen_def]>>
+  every_case_tac>>
+  simp[reify_avar_def,reify_reif_def,cmpop_val_def]>>
+  intLib.ARITH_TAC
+QED
+
 Theorem encode_equal_sem_1:
   valid_assignment bnd wi ∧
   ALOOKUP cs name = SOME (Prim (Cmpop reif cmp X Y)) ∧
@@ -55,8 +65,11 @@ Theorem encode_equal_sem_1:
     (encode_equal bnd Zr X Y name)
 Proof
   rw[reify_sem_def,encode_equal_def]>>
-  gvs[reify_avar_def,reify_reif_def,reify_flag_def,reif_gen_def,
-    AllCasePreds(),iconstraint_sem_def,SF DNF_ss]>>
+  gvs[AllCasePreds()]
+  >-intLib.ARITH_TAC>>
+  rpt CONJ_TAC>>
+  rw[reify_avar_def,reify_reif_def,reify_flag_def,
+    lit_reify_avar_reif_gen,SF DNF_ss,encode_reif_gen_sem]>>
   intLib.ARITH_TAC
 QED
 
@@ -67,8 +80,9 @@ Theorem encode_equal_sem_2:
   reify_sem Zr wi
     (varc wi X = varc wi Y)
 Proof
-  rw[reify_sem_def,reif_gen_def,encode_equal_def]>>
-  every_case_tac>>gvs[]>>
+  rw[reify_sem_def,encode_equal_def,cmpop_val_def]>>
+  every_case_tac>>
+  gvs[cmpop_val_def,reif_gen_def,encode_reif_gen_sem]>>
   intLib.ARITH_TAC
 QED
 
@@ -121,10 +135,24 @@ Theorem encode_not_equal_sem_1:
   EVERY (λx. iconstraint_sem x (wi,reify_avar cs wi))
     (encode_not_equal bnd Zr X Y name)
 Proof
-  rw[reify_sem_def,reif_gen_def,encode_not_equal_def]>>
-  gvs[AllCasePreds(),reify_avar_def,reify_flag_def,reify_reif_def]
-  >- intLib.ARITH_TAC>>
-  simp[SF DNF_ss,reify_avar_def,reify_flag_def,reify_reif_def]>>
+  rw[reify_sem_def,encode_not_equal_def]>>
+  gvs[reify_avar_def,reify_reif_def,reify_flag_def,
+    lit_reify_avar_reif_gen,AllCasePreds(),SF DNF_ss]
+  >-intLib.ARITH_TAC>>
+  simp[CONJ_ASSOC,encode_reif_gen_sem]>>
+  qmatch_goalsub_abbrev_tac ‘(P ∧ Q1) ∨ (P ∧ Q2) ∨ (P ∧ Q3)’>>
+  ‘P ∧ (Q1 ∨ Q2 ∨ Q3)’ suffices_by simp[]>>
+  unabbrev_all_tac>>
+  CONJ_TAC
+  >~[‘¬cmpop_val _ _ _’]
+  >-(
+    rename1 ‘_ ∨ _ ∨ ¬P’>>
+    Cases_on ‘P’>>
+    simp[]>>
+    intLib.ARITH_TAC)>>
+  rename1 ‘cmpop_val cmp' _ _’>>
+  Cases_on ‘cmp'’>>
+  gvs[cmpop_val_def,reify_avar_def,reify_reif_def,reify_flag_def,reif_gen_def]>>
   intLib.ARITH_TAC
 QED
 
@@ -135,14 +163,29 @@ Theorem encode_not_equal_sem_2:
   reify_sem Zr wi
     (varc wi X ≠ varc wi Y)
 Proof
-  rw[reify_sem_def,reif_gen_def,encode_not_equal_def]>>
-  gvs[AllCasePreds(),reify_avar_def,reify_flag_def,reify_reif_def]>>
-  every_case_tac>>gvs[]
-  >- (
-    rename1`INR f`>>
-    Cases_on`wb (INR f)`>>gvs[]>>
-    intLib.ARITH_TAC)>>
-  intLib.ARITH_TAC
+  rw[encode_not_equal_def]>>
+  every_case_tac
+  >-(
+    gvs[EVERY_APPEND,reify_sem_def]>>
+    qmatch_asmsub_abbrev_tac ‘¬P’>>
+    Cases_on ‘P’>>
+    gs[]>>
+    intLib.ARITH_TAC)
+  >-(
+    gvs[EVERY_APPEND,reify_sem_def]>>
+    every_case_tac>>
+    strip_tac>>
+    rfs[encode_reif_gen_sem]>>
+    intLib.ARITH_TAC)
+  >-(
+    gvs[EVERY_APPEND,reify_sem_def]>>
+    every_case_tac>>
+    rw[]>>
+    rfs[encode_reif_gen_sem]>>
+    qmatch_asmsub_abbrev_tac ‘¬P’>>
+    Cases_on ‘P’>>
+    gs[]>>
+    intLib.ARITH_TAC)
 QED
 
 (* this encompasses ≥, >, ≤, < *)
@@ -170,19 +213,69 @@ Definition encode_order_cmpops_def:
       bimply_bits bnd [reif_gen Zc] constr
 End
 
+Theorem encode_reif_gen_reify_avar:
+    valid_assignment bnd wi ⇒
+    EVERY (λx. iconstraint_sem x (wi,reify_avar cs wi)) (encode_reif_gen bnd (Z,cmp,v))
+Proof
+  rw[]>>
+  simp[encode_reif_gen_sem]>>
+  simp[reify_avar_def,reify_reif_def,reif_gen_def]>>
+  Cases_on ‘cmp’>>
+  simp[reify_avar_def,reify_reif_def,cmpop_val_def]>>
+  intLib.ARITH_TAC
+QED
+
+Theorem encode_cmp_aux_cmpop_val:
+  cmp ≠ Equal ∧
+  cmp ≠ NotEqual ⇒
+  (iconstraint_sem (encode_cmp_aux cmp X Y) (wi,wb) ⇔
+  cmpop_val cmp (varc wi X) (varc wi Y))
+Proof
+  rw[cmpop_val_def,encode_cmp_aux_def]>>
+  every_case_tac>>
+  fs[]>>
+  intLib.ARITH_TAC
+QED
+
+Theorem cmpop_val_reif_gen:
+  cmpop_val z1 (varc wi z0) z2 ⇔
+    lit (reify_avar cs wi) (reif_gen (z0,z1,z2))
+Proof
+  simp[cmpop_val_def,reif_gen_def]>>
+  every_case_tac>>
+  simp[reify_avar_def,reify_reif_def]>>
+  intLib.ARITH_TAC
+QED
+
 Theorem encode_order_cmpops_sem_1:
   valid_assignment bnd wi ∧ cmp ≠ Equal ∧ cmp ≠ NotEqual ∧
   reify_sem Zr wi (cmpop_val cmp (varc wi X) (varc wi Y)) ⇒
   EVERY (λx. iconstraint_sem x (wi,reify_avar cs wi))
     (encode_order_cmpops bnd Zr cmp X Y)
 Proof
-  Cases_on ‘cmp’>>
-  rw[reify_sem_def,reif_gen_def,cmpop_val_def,
-    encode_order_cmpops_def,
-    iconstraint_sem_def,encode_cmp_aux_def]>>
-  every_case_tac>>
-  gvs[AllCasePreds(),reify_avar_def,reify_reif_def]>>
-  intLib.ARITH_TAC
+  rw[encode_order_cmpops_def]>>
+  every_case_tac
+  >-(
+    rw[encode_cmp_aux_def]>>
+    every_case_tac>>
+    fs[reify_sem_def,cmpop_val_def]>>
+    intLib.ARITH_TAC)>>
+  rename1 ‘reif_gen z’>>
+  PairCases_on ‘z’>>
+  simp[EVERY_APPEND,encode_reif_gen_reify_avar]>>
+  simp[encode_cmp_aux_cmpop_val]>>
+  fs[reify_sem_def]>>
+  pop_assum mp_tac
+  >-(
+    qmatch_goalsub_abbrev_tac ‘(P ⇒ _) ⇒ (Q ⇒ _)’>>
+    ‘P ⇔ Q’ suffices_by simp[]>>
+    unabbrev_all_tac>>
+    simp[cmpop_val_reif_gen])
+  >-(
+    qmatch_goalsub_abbrev_tac ‘(P ⇔ _) ⇒ (_ ⇔ Q)’>>
+    ‘P ⇔ Q’ suffices_by simp[]>>
+    unabbrev_all_tac>>
+    simp[cmpop_val_reif_gen])
 QED
 
 Theorem encode_order_cmpops_sem_2:
@@ -191,10 +284,17 @@ Theorem encode_order_cmpops_sem_2:
     (encode_order_cmpops bnd Zr cmp X Y) ⇒
   reify_sem Zr wi (cmpop_val cmp (varc wi X) (varc wi Y))
 Proof
-  rw[reify_sem_def,reif_gen_def,encode_order_cmpops_def,cmpop_val_def,encode_cmp_aux_def]>>
+  rw[encode_order_cmpops_def]>>
+  every_case_tac
+  >-(
+    fs[reify_sem_def,encode_cmp_aux_def,cmpop_val_def]>>
+    every_case_tac>>
+    fs[iconstraint_sem_def]>>
+    intLib.ARITH_TAC)>>
+  simp[reify_sem_def]>>
   every_case_tac>>
-  gvs[]>>
-  intLib.ARITH_TAC
+  gvs[EVERY_APPEND,encode_reif_gen_sem]>>
+  metis_tac[encode_cmp_aux_cmpop_val]
 QED
 
 (* -X ≥ Y *)
